src/ArrayList.fsti
@@ -13,7 +13,30 @@ module US = FStar.SizeT
 module FS = FStar.FiniteSet.Base
 module AL = ArrayListGen
 
-let read_in_place
+(** A monomorphized version of ArrayListGen, specialized for cells of statuses, i.e., 0ul, 1ul, or 2ul.
+    We only expose the computationally relevant functions here, all the lemmas remain in ArrayListGen *)
+
+inline_for_extraction noextract
+let status = v:U32.t{U32.v v < 3}
+
+let cell : Type0 = AL.cell status
+
+inline_for_extraction noextract
+let null = AL.null
+inline_for_extraction noextract
+let null_ptr = AL.null_ptr
+
+unfold
+let varraylist (pred1 pred2 pred3: status -> prop) (r:A.array cell) (hd1 hd2 hd3:nat) : vprop =
+  AL.varraylist pred1 pred2 pred3 r hd1 hd2 hd3
+
+[@@ __steel_reduce__]
+let v_arraylist (#p2:vprop) (pred1 pred2 pred3: status -> prop) (r:A.array cell) (hd1 hd2 hd3:nat)
+  (h:rmem p2{FStar.Tactics.with_tactic selector_tactic
+    (can_be_split p2 (varraylist pred1 pred2 pred3 r hd1 hd2 hd3) /\ True)}) : GTot (Seq.seq cell)
+  = h (varraylist pred1 pred2 pred3 r hd1 hd2 hd3)
+
+val read_in_place
   (#pred1 #pred2 #pred3: status -> prop)
   (r:A.array cell)
   (hd1 hd2 hd3:Ghost.erased nat)
@@ -26,12 +49,13 @@ let read_in_place
             result == AL.get_data (Seq.index (v_arraylist pred1 pred2 pred3 r hd1 hd2 hd3 h0) (US.v idx)) /\
             h0 (varraylist pred1 pred2 pred3 r hd1 hd2 hd3) ==
             h1 (varraylist pred1 pred2 pred3 r hd1 hd2 hd3))
-  =
-  admit ();
-  AL.read_in_place r hd1 hd2 hd3 idx
 
 /// Removes the element at offset [idx] from the dlist pointed to by [hd1]
-let remove
+/// We provide three variants for simplicity of use, and perform the permutations
+/// of the lists in the varraylist predicate internally to only expose one idiomatic
+/// remove function
+inline_for_extraction noextract
+val remove1
   (#pred1 #pred2 #pred3: status -> prop)
   (r:A.array cell)
   (hd1:US.t)
@@ -52,35 +76,9 @@ let remove
             AL.dataify (h1 (varraylist pred1 pred2 pred3 r (US.v hd') hd2 hd3)) ==
             AL.dataify (h0 (varraylist pred1 pred2 pred3 r (US.v hd1) hd2 hd3))
           )
-  = AL.remove r hd1 hd2 hd3 idx
-
-/// Removes the element at offset [idx] from the dlist pointed to by [hd1]
-inline_for_extraction noextract
-let remove1
-  (#pred1 #pred2 #pred3: status -> prop)
-  (r:A.array cell)
-  (hd1:US.t)
-  (hd2 hd3:Ghost.erased nat)
-  (idx:US.t{US.v idx < A.length r})
-   : Steel US.t
-          (varraylist pred1 pred2 pred3 r (US.v hd1) hd2 hd3)
-          (fun hd' -> varraylist pred1 pred2 pred3 r (US.v hd') hd2 hd3)
-          (requires fun h -> AL.mem (US.v idx) (US.v hd1) (h (varraylist pred1 pred2 pred3 r (US.v hd1) hd2 hd3)))
-          (ensures fun h0 hd' h1 ->
-            AL.ptrs_in (US.v hd') (h1 (varraylist pred1 pred2 pred3 r (US.v hd') hd2 hd3)) ==
-            FS.remove (US.v idx) (AL.ptrs_in (US.v hd1) (h0 (varraylist pred1 pred2 pred3 r (US.v hd1) hd2 hd3))) /\
-            AL.ptrs_in hd2 (h1 (varraylist pred1 pred2 pred3 r (US.v hd') hd2 hd3)) ==
-            AL.ptrs_in hd2 (h0 (varraylist pred1 pred2 pred3 r (US.v hd1) hd2 hd3)) /\
-            AL.ptrs_in hd3 (h1 (varraylist pred1 pred2 pred3 r (US.v hd') hd2 hd3)) ==
-            AL.ptrs_in hd3 (h0 (varraylist pred1 pred2 pred3 r (US.v hd1) hd2 hd3)) /\
-            (~ (AL.mem_all (US.v idx) (US.v hd') hd2 hd3 (h1 (varraylist pred1 pred2 pred3 r (US.v hd') hd2 hd3)))) /\
-            AL.dataify (h1 (varraylist pred1 pred2 pred3 r (US.v hd') hd2 hd3)) ==
-            AL.dataify (h0 (varraylist pred1 pred2 pred3 r (US.v hd1) hd2 hd3))
-          )
-  = remove r hd1 hd2 hd3 idx
 
 inline_for_extraction noextract
-let remove2
+val remove2
   (#pred1 #pred2 #pred3: status -> prop)
   (r:A.array cell)
   (hd1:Ghost.erased nat)
@@ -102,13 +100,9 @@ let remove2
             AL.dataify (h1 (varraylist pred1 pred2 pred3 r hd1 (US.v hd') hd3)) ==
             AL.dataify (h0 (varraylist pred1 pred2 pred3 r hd1 (US.v hd2) hd3))
           )
-  = AL.permute12 pred1 pred2 pred3 r hd1 (US.v hd2) hd3;
-    let v = remove r hd2 hd1 hd3 idx in
-    AL.permute12 pred2 pred1 pred3 r (US.v v) hd1 hd3;
-    return v
 
 inline_for_extraction noextract
-let remove3
+val remove3
   (#pred1 #pred2 #pred3: status -> prop)
   (r:A.array cell)
   (hd1:Ghost.erased nat)
@@ -130,12 +124,9 @@ let remove3
             AL.dataify (h1 (varraylist pred1 pred2 pred3 r hd1 hd2 (US.v hd'))) ==
             AL.dataify (h0 (varraylist pred1 pred2 pred3 r hd1 hd2 (US.v hd3)))
           )
-  = AL.permute13 pred1 pred2 pred3 r hd1 hd2 (US.v hd3);
-    let v = remove r hd3 hd2 hd1 idx in
-    AL.permute13 pred3 pred2 pred1 r (US.v v) hd2 hd1;
-    return v
 
-let insert
+inline_for_extraction noextract
+val insert1
   (#pred1 #pred2 #pred3: status -> prop)
   (r:A.array cell)
   (hd:US.t)
@@ -157,33 +148,9 @@ let insert
             AL.dataify (h1 (varraylist pred1 pred2 pred3 r (US.v idx) hd2 hd3)) ==
             Seq.upd (AL.dataify (h0 (varraylist pred1 pred2 pred3 r (US.v hd) hd2 hd3))) (US.v idx) v
           )
-  = AL.insert r hd hd2 hd3 idx v
 
-let insert1
-  (#pred1 #pred2 #pred3: status -> prop)
-  (r:A.array cell)
-  (hd:US.t)
-  (hd2 hd3:Ghost.erased nat)
-  (idx:US.t{idx <> null_ptr /\ US.v idx < A.length r})
-  (v: status)
-   : Steel unit
-          (varraylist pred1 pred2 pred3 r (US.v hd) hd2 hd3)
-          (fun _ -> varraylist pred1 pred2 pred3 r (US.v idx) hd2 hd3)
-          (requires fun h -> pred1 v /\
-            (~ (AL.mem_all (US.v idx) (US.v hd) hd2 hd3 (h (varraylist pred1 pred2 pred3 r (US.v hd) hd2 hd3)))))
-          (ensures fun h0 hd' h1 ->
-            AL.ptrs_in (US.v idx) (h1 (varraylist pred1 pred2 pred3 r (US.v idx) hd2 hd3)) ==
-            FS.insert (US.v idx) (AL.ptrs_in (US.v hd) (h0 (varraylist pred1 pred2 pred3 r (US.v hd) hd2 hd3))) /\
-            AL.ptrs_in hd2 (h1 (varraylist pred1 pred2 pred3 r (US.v idx) hd2 hd3)) ==
-            AL.ptrs_in hd2 (h0 (varraylist pred1 pred2 pred3 r (US.v hd) hd2 hd3)) /\
-            AL.ptrs_in hd3 (h1 (varraylist pred1 pred2 pred3 r (US.v idx) hd2 hd3)) ==
-            AL.ptrs_in hd3 (h0 (varraylist pred1 pred2 pred3 r (US.v hd) hd2 hd3)) /\
-            AL.dataify (h1 (varraylist pred1 pred2 pred3 r (US.v idx) hd2 hd3)) ==
-            Seq.upd (AL.dataify (h0 (varraylist pred1 pred2 pred3 r (US.v hd) hd2 hd3))) (US.v idx) v
-          )
-  = insert r hd hd2 hd3 idx v
-
-let insert2
+inline_for_extraction noextract
+val insert2
   (#pred1 #pred2 #pred3: status -> prop)
   (r:A.array cell)
   (hd:US.t)
@@ -205,11 +172,9 @@ let insert2
             AL.dataify (h1 (varraylist pred1 pred2 pred3 r hd1 (US.v idx) hd3)) ==
             Seq.upd (AL.dataify (h0 (varraylist pred1 pred2 pred3 r hd1 (US.v hd) hd3))) (US.v idx) v
           )
-  = AL.permute12 pred1 pred2 pred3 r hd1 (US.v hd) hd3;
-    insert r hd hd1 hd3 idx v;
-    AL.permute12 pred2 pred1 pred3 r (US.v idx) hd1 hd3
 
-let insert3
+inline_for_extraction noextract
+val insert3
   (#pred1 #pred2 #pred3: status -> prop)
   (r:A.array cell)
   (hd:US.t)
@@ -231,34 +196,9 @@ let insert3
             AL.dataify (h1 (varraylist pred1 pred2 pred3 r hd1 hd2 (US.v idx))) ==
             Seq.upd (AL.dataify (h0 (varraylist pred1 pred2 pred3 r hd1 hd2 (US.v hd)))) (US.v idx) v
           )
-  = AL.permute13 pred1 pred2 pred3 r hd1 hd2 (US.v hd);
-    insert r hd hd2 hd1 idx v;
-    AL.permute13 pred3 pred2 pred1 r (US.v idx) hd2 hd1
-
-let extend
-  (#pred1 #pred2 #pred3: status -> prop)
-  (r:A.array cell)
-  (hd:US.t{hd == null_ptr \/ US.v hd < A.length r})
-  (hd2 hd3:Ghost.erased nat)
-  (k:US.t{US.v k + 1 <= A.length r /\ US.fits (US.v k + 1)})
-  (v: status)
-  : Steel unit
-          (AL.varraylist pred1 pred2 pred3 (A.split_l r k) (US.v hd) hd2 hd3 `star`
-            A.varray (A.split_l (A.split_r r k) 1sz))
-          (fun _ ->
-            AL.varraylist pred1 pred2 pred3 (A.split_l r (k `US.add` 1sz)) (US.v k) hd2 hd3)
-          (requires fun _ ->
-            k <> null_ptr /\ pred1 v)
-          (ensures fun h0 _ h1 ->
-            A.length_fits r;
-            AL.dataify (h1 (varraylist pred1 pred2 pred3 (A.split_l r (k `US.add` 1sz)) (US.v k) hd2 hd3))
-              `Seq.equal`
-            Seq.append (AL.dataify (h0 (varraylist pred1 pred2 pred3 (A.split_l r k) (US.v hd) hd2 hd3))) (Seq.create 1 v)
-          )
-  = AL.extend r hd hd2 hd3 k v
 
 inline_for_extraction noextract
-let extend1
+val extend1
   (#pred1 #pred2 #pred3: status -> prop)
   (r:A.array cell)
   (hd:US.t{hd == null_ptr \/ US.v hd < A.length r})
@@ -278,4 +218,3 @@ let extend1
               `Seq.equal`
             Seq.append (AL.dataify (h0 (varraylist pred1 pred2 pred3 (A.split_l r k) (US.v hd) hd2 hd3))) (Seq.create 1 v)
           )
-  = extend r hd hd2 hd3 k v
